theories/Machine.v
@@ -120,6 +120,8 @@ Module MinCapsTermKit <: TermKit.
   Inductive Lem : PCtx -> Set :=
   | open_ptsreg                : Lem ["reg" ∶ ty_enum regname]
   | close_ptsreg (R : RegName) : Lem ctx.nil
+  | open_gprs                  : Lem ctx.nil
+  | close_gprs                 : Lem ctx.nil
   | safe_move_cursor           : Lem ["c'" ∶ ty_cap, "c" ∶ ty_cap]
   | safe_sub_perm              : Lem ["c'" ∶ ty_cap, "c" ∶ ty_cap]
   | safe_within_range          : Lem ["c'" ∶ ty_cap, "c" ∶ ty_cap]
@@ -229,8 +231,8 @@ Module MinCapsProgramKit <: (ProgramKit MinCapsTermKit).
     match: exp_var "rreg" in regname with
     | R0 => let: "x" := stm_read_register reg0 in use lemma (close_ptsreg R0) ;; stm_exp x
     | R1 => let: "x" := stm_read_register reg1 in use lemma (close_ptsreg R1) ;; stm_exp x
-    (* | R2 => let: "x" := stm_read_register reg2 in use lemma (close_ptsreg R2) ;; stm_exp x
-    | R3 => let: "x" := stm_read_register reg3 in use lemma (close_ptsreg R3) ;; stm_exp x *)
+    | R2 => let: "x" := stm_read_register reg2 in use lemma (close_ptsreg R2) ;; stm_exp x
+    | R3 => let: "x" := stm_read_register reg3 in use lemma (close_ptsreg R3) ;; stm_exp x
     end.
 
   Definition fun_read_reg_cap : Stm ["creg" ∶ ty_enum regname ] ty_cap :=
@@ -254,9 +256,10 @@ Module MinCapsProgramKit <: (ProgramKit MinCapsTermKit).
     match: exp_var "wreg" in regname with
     | R0 => let: "x" := stm_write_register reg0 (exp_var "w") in use lemma (close_ptsreg R0) ;; stm_exp x
     | R1 => let: "x" := stm_write_register reg1 (exp_var "w") in use lemma (close_ptsreg R1) ;; stm_exp x
-    (* | R2 => let: "x" := stm_write_register reg2 (exp_var "w") in use lemma (close_ptsreg R2) ;; stm_exp x *)
-    (* | R3 => let: "x" := stm_write_register reg3 (exp_var "w") in use lemma (close_ptsreg R3) ;; stm_exp x *)
-    end ;; stm_val ty_unit tt.
+    | R2 => let: "x" := stm_write_register reg2 (exp_var "w") in use lemma (close_ptsreg R2) ;; stm_exp x
+    | R3 => let: "x" := stm_write_register reg3 (exp_var "w") in use lemma (close_ptsreg R3) ;; stm_exp x
+    end ;;
+    stm_val ty_unit tt.
 
   Definition fun_next_pc : Stm ctx.nil ty_cap :=
     let: "c" := stm_read_register pc in
@@ -322,6 +325,7 @@ Module MinCapsProgramKit <: (ProgramKit MinCapsTermKit).
     Definition fun_exec_sd : Stm [hv ∶ ty_hv, lv ∶ ty_lv, "immediate" ∶ ty_int ] ty_bool :=
       stm_match_enum regname (exp_var "lv") (fun _ => stm_val ty_unit tt) ;;
       stm_match_enum regname (exp_var "hv") (fun _ => stm_val ty_unit tt) ;;
+      use lemma open_gprs ;;
       let: "base_cap" :: cap  := call read_reg_cap lv in
       let*: ["perm", "beg", "end", "cursor"] := (exp_var "base_cap") in
       (let: "c" :: cap := exp_record capability
@@ -331,6 +335,7 @@ Module MinCapsProgramKit <: (ProgramKit MinCapsTermKit).
                                        exp_var "cursor" + exp_var "immediate"
                                      ] in
        let: w :: ty_word := call read_reg hv in
+       use lemma close_gprs ;;
        use lemma safe_move_cursor [exp_var "c", exp_var "base_cap"] ;;
        call write_mem c w ;;
        call update_pc ;;
@@ -338,6 +343,7 @@ Module MinCapsProgramKit <: (ProgramKit MinCapsTermKit).
 
     Definition fun_exec_ld : Stm [lv ∶ ty_lv, hv ∶ ty_hv, "immediate" ∶ ty_int ] ty_bool :=
       stm_match_enum regname (exp_var "hv") (fun _ => stm_val ty_unit tt) ;;
+      use lemma open_gprs ;;
       let: "base_cap" :: cap  := call read_reg_cap hv in
       let*: ["perm", "beg", "end", "cursor"] := (exp_var "base_cap") in
       (let: "c" :: cap := exp_record capability
@@ -350,12 +356,14 @@ Module MinCapsProgramKit <: (ProgramKit MinCapsTermKit).
        let: n :: ty_memval := call read_mem c in
        stm_match_enum regname (exp_var "lv") (fun _ => stm_val ty_unit tt) ;;
        call write_reg lv (exp_var n) ;;
+       use lemma close_gprs ;;
        call update_pc ;;
        stm_val ty_bool true).
 
     Definition fun_exec_lea : Stm ["lv" ∶ ty_lv, "hv" ∶ ty_hv] ty_bool :=
       stm_match_enum regname (exp_var "lv") (fun _ => stm_val ty_unit tt) ;;
       stm_match_enum regname (exp_var "hv") (fun _ => stm_val ty_unit tt) ;;
+      use lemma open_gprs ;;
       let: "base_cap" :: cap  := call read_reg_cap (exp_var "lv") in
       let: "offset" :: ty_int := call read_reg_num (exp_var "hv") in
       let*: ["perm", "beg", "end", "cursor"] := (exp_var "base_cap") in
@@ -367,12 +375,14 @@ Module MinCapsProgramKit <: (ProgramKit MinCapsTermKit).
                                      ] in
        use lemma safe_move_cursor [exp_var "c", exp_var "base_cap"] ;;
        call write_reg (exp_var "lv") (exp_inr (exp_var "c")) ;;
+       use lemma close_gprs ;;
        call update_pc ;;
        stm_val ty_bool true).
 
     Definition fun_exec_restrict : Stm ["lv" ∶ ty_lv, "hv" ∶ ty_hv] ty_bool :=
       stm_match_enum regname (exp_var "lv") (fun _ => stm_val ty_unit tt) ;;
       stm_match_enum regname (exp_var "hv") (fun _ => stm_val ty_unit tt) ;;
+      use lemma open_gprs ;;
       let: "c" :: cap  := call read_reg_cap (exp_var "lv") in
       let: "n" :: ty_int := call read_reg_num (exp_var "hv") in
       let*: ["p", "beg", "end", "cursor"] := (exp_var "c") in
@@ -387,11 +397,13 @@ Module MinCapsProgramKit <: (ProgramKit MinCapsTermKit).
                                       ] in
        use lemma safe_sub_perm [exp_var "c'", exp_var "c"] ;;
        call write_reg (exp_var "lv") (exp_inr (exp_var "c'")) ;;
+       use lemma close_gprs ;;
        call update_pc ;;
        stm_val ty_bool true).
 
     Definition fun_exec_restricti : Stm ["lv" ∶ ty_lv, "immediate" ∶ ty_int] ty_bool :=
       stm_match_enum regname (exp_var "lv") (fun _ => stm_val ty_unit tt) ;;
+      use lemma open_gprs ;;
       let: "c" :: cap  := call read_reg_cap (exp_var "lv") in
       let: "n" :: ty_int := exp_var "immediate" in
       let*: ["p", "beg", "end", "cursor"] := (exp_var "c") in
@@ -406,40 +418,47 @@ Module MinCapsProgramKit <: (ProgramKit MinCapsTermKit).
                                       ] in
        use lemma safe_sub_perm [exp_var "c'", exp_var "c"] ;;
        call write_reg (exp_var "lv") (exp_inr (exp_var "c'")) ;;
+       use lemma close_gprs ;;
        call update_pc ;;
        stm_val ty_bool true).
 
     Definition fun_exec_addi : Stm ["lv" ∶ ty_lv, "hv" ∶ ty_hv, "immediate" ∶ ty_int ] ty_bool :=
       stm_match_enum regname (exp_var "hv") (fun _ => stm_val ty_unit tt) ;;
+      use lemma open_gprs ;;
       let: "v" :: ty_int := call read_reg_num (exp_var "hv") in
       let: "res" :: ty_int := stm_exp (exp_var "v" + exp_var "immediate") in
       stm_match_enum regname (exp_var "lv") (fun _ => stm_val ty_unit tt) ;;
       call write_reg (exp_var "lv") (exp_inl (exp_var "res")) ;;
       use lemma int_safe [exp_var "res"] ;;
+      use lemma close_gprs ;;
       call update_pc ;;
       stm_val ty_bool true.
 
     Definition fun_exec_add : Stm ["lv1" ∶ ty_lv, "lv2" ∶ ty_lv, "lv3" ∶ ty_lv ] ty_bool :=
       stm_match_enum regname (exp_var "lv2") (fun _ => stm_val ty_unit tt) ;;
       stm_match_enum regname (exp_var "lv3") (fun _ => stm_val ty_unit tt) ;;
+      use lemma open_gprs ;;
       let: "v1" :: int := call read_reg_num (exp_var "lv2") in
       let: "v2" :: int := call read_reg_num (exp_var "lv3") in
       let: "res" :: int := stm_exp (exp_var "v1" + exp_var "v2") in
       stm_match_enum regname (exp_var "lv1") (fun _ => stm_val ty_unit tt) ;;
       call write_reg (exp_var "lv1") (exp_inl (exp_var "res")) ;;
       use lemma int_safe [exp_var "res"] ;;
+      use lemma close_gprs ;;
       call update_pc ;;
       stm_val ty_bool true.
 
     Definition fun_exec_sub : Stm ["lv1" ∶ ty_lv, "lv2" ∶ ty_lv, "lv3" ∶ ty_lv] ty_bool :=
       stm_match_enum regname (exp_var "lv2") (fun _ => stm_val ty_unit tt) ;;
       stm_match_enum regname (exp_var "lv3") (fun _ => stm_val ty_unit tt) ;;
+      use lemma open_gprs ;;
       let: "v1" :: int := call read_reg_num (exp_var "lv2") in
       let: "v2" :: int := call read_reg_num (exp_var "lv3") in
       let: "res" :: int := stm_exp (exp_var "v1" - exp_var "v2") in
       stm_match_enum regname (exp_var "lv1") (fun _ => stm_val ty_unit tt) ;;
       call write_reg (exp_var "lv1") (exp_inl (exp_var "res")) ;;
       use lemma int_safe [exp_var "res"] ;;
+      use lemma close_gprs ;;
       call update_pc ;;
       stm_val ty_bool true.
 
@@ -451,6 +470,7 @@ Module MinCapsProgramKit <: (ProgramKit MinCapsTermKit).
     Definition fun_exec_slt : Stm ["lv1" ∶ ty_lv, "lv2" ∶ ty_lv, "lv3" ∶ ty_lv] ty_bool :=
       stm_match_enum regname (exp_var "lv2") (fun _ => stm_val ty_unit tt) ;;
       stm_match_enum regname (exp_var "lv3") (fun _ => stm_val ty_unit tt) ;;
+      use lemma open_gprs ;;
       let: "v1" :: int := call read_reg_num (exp_var "lv2") in
       let: "v2" :: int := call read_reg_num (exp_var "lv3") in
       stm_match_enum regname (exp_var "lv1") (fun _ => stm_val ty_unit tt) ;;
@@ -461,11 +481,13 @@ Module MinCapsProgramKit <: (ProgramKit MinCapsTermKit).
        else
          call write_reg (exp_var "lv1") (exp_inl (exp_val ty_int 0%Z)) ;;
          use lemma int_safe [exp_val ty_int 0%Z]) ;;
+      use lemma close_gprs ;;
       call update_pc ;;
       stm_val ty_bool true.
 
     Definition fun_exec_slti : Stm ["lv" ∶ ty_lv, "hv" ∶ ty_hv, "immediate" ∶ ty_int ] ty_bool :=
       stm_match_enum regname (exp_var "hv") (fun _ => stm_val ty_unit tt) ;;
+      use lemma open_gprs ;;
       let: "v1" :: int := call read_reg_num (exp_var "hv") in
       let: "v2" :: int := exp_var "immediate" in
       stm_match_enum regname (exp_var "lv") (fun _ => stm_val ty_unit tt) ;;
@@ -476,12 +498,14 @@ Module MinCapsProgramKit <: (ProgramKit MinCapsTermKit).
        else
          call write_reg (exp_var "lv") (exp_inl (exp_val ty_int 0%Z)) ;;
          use lemma int_safe [exp_val ty_int 0%Z]) ;;
+      use lemma close_gprs ;;
       call update_pc ;;
       stm_val ty_bool true.
 
     Definition fun_exec_sltu : Stm ["lv1" ∶ ty_lv, "lv2" ∶ ty_lv, "lv3" ∶ ty_lv] ty_bool :=
       stm_match_enum regname (exp_var "lv2") (fun _ => stm_val ty_unit tt) ;;
       stm_match_enum regname (exp_var "lv3") (fun _ => stm_val ty_unit tt) ;;
+      use lemma open_gprs ;;
       let: "v1" :: int := call read_reg_num (exp_var "lv2") in
       let: "uv1" :: int := call abs (exp_var "v1") in
       let: "v2" :: int := call read_reg_num (exp_var "lv3") in
@@ -494,11 +518,13 @@ Module MinCapsProgramKit <: (ProgramKit MinCapsTermKit).
        else
          call write_reg (exp_var "lv1") (exp_inl (exp_val ty_int 0%Z)) ;;
          use lemma int_safe [exp_val ty_int 0%Z]) ;;
+      use lemma close_gprs ;;
       call update_pc ;;
       stm_val ty_bool true.
 
     Definition fun_exec_sltiu : Stm ["lv" ∶ ty_lv, "hv" ∶ ty_hv, "immediate" ∶ ty_int ] ty_bool :=
       stm_match_enum regname (exp_var "hv") (fun _ => stm_val ty_unit tt) ;;
+      use lemma open_gprs ;;
       let: "v1" :: int := call read_reg_num (exp_var "hv") in
       let: "uv1" :: int := call abs (exp_var "v1") in
       let: "v2" :: int := exp_var "immediate" in
@@ -511,6 +537,7 @@ Module MinCapsProgramKit <: (ProgramKit MinCapsTermKit).
        else
          call write_reg (exp_var "lv") (exp_inl (exp_val ty_int 0%Z)) ;;
          use lemma int_safe [exp_val ty_int 0%Z]) ;;
+      use lemma close_gprs ;;
       call update_pc ;;
       stm_val ty_bool true.
 
@@ -553,6 +580,7 @@ Module MinCapsProgramKit <: (ProgramKit MinCapsTermKit).
       stm_match_enum regname (exp_var "lv") (fun _ => stm_val ty_unit tt) ;;
       stm_match_enum regname (exp_var "hv1") (fun _ => stm_val ty_unit tt) ;;
       stm_match_enum regname (exp_var "hv2") (fun _ => stm_val ty_unit tt) ;;
+      use lemma open_gprs ;;
       let: c :: cap := call read_reg_cap (exp_var "lv") in
       let: "new_begin" :: ty_int := call read_reg_num (exp_var "hv1") in
       let: "new_end" :: ty_int := call read_reg_num (exp_var "hv2") in
@@ -569,6 +597,7 @@ Module MinCapsProgramKit <: (ProgramKit MinCapsTermKit).
        use lemma gen_dummy [exp_var "c'"] ;;
        use lemma safe_within_range [exp_var "c'", exp_var "c"] ;;
        call write_reg (exp_var "lv") (exp_inr (exp_var "c'")) ;;
+       use lemma close_gprs ;;
        call update_pc ;;
        stm_val ty_bool true).
 
@@ -576,6 +605,7 @@ Module MinCapsProgramKit <: (ProgramKit MinCapsTermKit).
                                       ty_bool :=
       stm_match_enum regname (exp_var "lv") (fun _ => stm_val ty_unit tt) ;;
       stm_match_enum regname (exp_var "hv") (fun _ => stm_val ty_unit tt) ;;
+      use lemma open_gprs ;;
       let: c :: cap := call read_reg_cap (exp_var "lv") in
       let: "new_begin" :: ty_int := call read_reg_num (exp_var "hv") in
       let: "new_end" :: ty_int := exp_var "immediate" in
@@ -592,12 +622,14 @@ Module MinCapsProgramKit <: (ProgramKit MinCapsTermKit).
        use lemma gen_dummy [exp_var "c'"] ;;
        use lemma safe_within_range [exp_var "c'", exp_var "c"] ;;
        call write_reg (exp_var "lv") (exp_inr (exp_var "c'")) ;;
+       use lemma close_gprs ;;
        call update_pc ;;
        stm_val ty_bool true).
 
     Definition fun_exec_isptr : Stm ["lv1" ∶ ty_lv, "lv2" ∶ ty_lv] ty_bool :=
       stm_match_enum regname (exp_var "lv1") (fun _ => stm_val ty_unit tt) ;;
       stm_match_enum regname (exp_var "lv2") (fun _ => stm_val ty_unit tt) ;;
+      use lemma open_gprs ;;
       let: w :: ty_word := call read_reg (exp_var "lv2") in
       match: w with
       | inl i =>
@@ -607,47 +639,56 @@ Module MinCapsProgramKit <: (ProgramKit MinCapsTermKit).
         use lemma int_safe [exp_val ty_int 1%Z] ;;
         call write_reg (exp_var "lv1") (exp_inl (exp_val ty_int 1%Z))
       end ;;
+      use lemma close_gprs ;;
       call update_pc ;;
       stm_val ty_bool true.
 
     Definition fun_exec_getp : Stm ["lv1" ∶ ty_lv, "lv2" ∶ ty_lv] ty_bool :=
       stm_match_enum regname (exp_var "lv1") (fun _ => stm_val ty_unit tt) ;;
       stm_match_enum regname (exp_var "lv2") (fun _ => stm_val ty_unit tt) ;;
+      use lemma open_gprs ;;
       let: c :: cap := call read_reg_cap (exp_var "lv2") in
       let*: ["perm", "beg", "end", "cursor"] := (exp_var "c") in
       (let: "i" :: ty_int := call perm_to_bits (exp_var "perm") in
        call write_reg (exp_var "lv1") (exp_inl (exp_var "i")) ;;
        use lemma int_safe [exp_var "i"] ;;
+       use lemma close_gprs ;;
        call update_pc ;;
        stm_val ty_bool true).
 
     Definition fun_exec_getb : Stm ["lv1" ∶ ty_lv, "lv2" ∶ ty_lv] ty_bool :=
       stm_match_enum regname (exp_var "lv1") (fun _ => stm_val ty_unit tt) ;;
       stm_match_enum regname (exp_var "lv2") (fun _ => stm_val ty_unit tt) ;;
+      use lemma open_gprs ;;
       let: c :: cap := call read_reg_cap (exp_var "lv2") in
       let*: ["perm", "beg", "end", "cursor"] := (exp_var "c") in
       (call write_reg (exp_var "lv1") (exp_inl (exp_var "beg")) ;;
        use lemma int_safe [exp_var "beg"] ;;
+       use lemma close_gprs ;;
        call update_pc ;;
        stm_val ty_bool true).
 
     Definition fun_exec_gete : Stm ["lv1" ∶ ty_lv, "lv2" ∶ ty_lv] ty_bool :=
       stm_match_enum regname (exp_var "lv1") (fun _ => stm_val ty_unit tt) ;;
       stm_match_enum regname (exp_var "lv2") (fun _ => stm_val ty_unit tt) ;;
+      use lemma open_gprs ;;
       let: c :: cap := call read_reg_cap (exp_var "lv2") in
       let*: ["perm", "beg", "end", "cursor"] := (exp_var "c") in
       (call write_reg (exp_var "lv1") (exp_inl (exp_var "end")) ;;
        use lemma int_safe [exp_var "end"] ;;
+       use lemma close_gprs ;;
        call update_pc ;;
        stm_val ty_bool true).
 
     Definition fun_exec_geta : Stm ["lv1" ∶ ty_lv, "lv2" ∶ ty_lv] ty_bool :=
       stm_match_enum regname (exp_var "lv1") (fun _ => stm_val ty_unit tt) ;;
       stm_match_enum regname (exp_var "lv2") (fun _ => stm_val ty_unit tt) ;;
+      use lemma open_gprs ;;
       let: c :: cap := call read_reg_cap (exp_var "lv2") in
       let*: ["perm", "beg", "end", "cursor"] := (exp_var "c") in
       (call write_reg (exp_var "lv1") (exp_inl (exp_var "cursor")) ;;
        use lemma int_safe [exp_var "cursor"] ;;
+       use lemma close_gprs ;;
        call update_pc ;;
        stm_val ty_bool true).
 
@@ -660,15 +701,19 @@ Module MinCapsProgramKit <: (ProgramKit MinCapsTermKit).
     Definition fun_exec_mv : Stm [lv ∶ ty_lv, hv ∶ ty_hv] ty_bool :=
       stm_match_enum regname (exp_var "hv") (fun _ => stm_val ty_unit tt) ;;
       stm_match_enum regname (exp_var "lv") (fun _ => stm_val ty_unit tt) ;;
+      use lemma open_gprs ;;
       let: w :: word := call read_reg (exp_var hv) in
       call write_reg lv (exp_var w) ;;
+      use lemma close_gprs ;;
       call update_pc ;;
       stm_val ty_bool true.
 
     Definition fun_exec_jr : Stm ["lv" ∶ ty_lv] ty_bool :=
       stm_match_enum regname (exp_var "lv") (fun _ => stm_val ty_unit tt) ;;
+      use lemma open_gprs ;;
       let: "c" :: ty_cap := call read_reg_cap (exp_var "lv") in
       stm_write_register pc (exp_var "c") ;;
+      use lemma close_gprs ;;
       stm_val ty_bool true.
 
     Definition fun_exec_jalr : Stm ["lv1" ∶ ty_lv, "lv2" ∶ ty_lv] ty_bool :=
@@ -676,7 +721,9 @@ Module MinCapsProgramKit <: (ProgramKit MinCapsTermKit).
       let: "npc" := call next_pc in
       use lemma safe_move_cursor [exp_var "npc", exp_var "opc"] ;;
       stm_match_enum regname (exp_var "lv1") (fun _ => stm_val ty_unit tt) ;;
+      use lemma open_gprs ;;
       call write_reg (exp_var "lv1") (exp_inr (exp_var "npc")) ;;
+      use lemma close_gprs ;;
       call exec_jr (exp_var "lv2").
 
     Definition fun_exec_j : Stm [offset ∶ ty_int ] ty_bool :=
@@ -688,12 +735,16 @@ Module MinCapsProgramKit <: (ProgramKit MinCapsTermKit).
       let: "npc" := call next_pc in
       use lemma safe_move_cursor [exp_var "npc", exp_var "opc"] ;;
       stm_match_enum regname (exp_var "lv") (fun _ => stm_val ty_unit tt) ;;
+      use lemma open_gprs ;;
       call write_reg lv (exp_inr (exp_var "npc")) ;;
+      use lemma close_gprs ;;
       call exec_j offset.
 
     Definition fun_exec_bnez : Stm ["lv" ∶ ty_lv, "immediate" ∶ ty_int ] ty_bool :=
       stm_match_enum regname (exp_var "lv") (fun _ => stm_val ty_unit tt) ;;
+      use lemma open_gprs ;;
       let: "c" :: ty_int := call read_reg_num (exp_var "lv") in
+      use lemma close_gprs ;;
       stm_if (exp_binop binop_eq (exp_var "c") (exp_int 0))
              (call update_pc ;; stm_val ty_bool true)
              (call add_pc (exp_var "immediate") ;; stm_val ty_bool true).
